Implementation.v
@@ -90,19 +90,22 @@ Fixpoint single_exit_point (C:Choreography) : Prop :=
   end.
 
 Lemma fatsemi_precongr : forall C C1 C2, C1 ~<= C2 -> (C1;;C) ~<= (C2;;C).
+Proof.
 intros; induction H.
-- apply Refl.
-- apply Trans with (C2;;C); auto; clear C3 H0 IHPrecongr.
-- apply EtaEta; auto.
-- apply EtaCond; auto.
-- apply CondEta; auto.
-- apply CondCond; auto.
-- apply CtxEta; auto.
-- apply CtxThen; auto.
-- apply CtxElse; auto.
++ apply Refl.
++ apply Trans with (C2;;C); auto; clear C3 H0 IHPrecongr.
+  induction H.
+  - apply EtaEta; auto.
+  - apply EtaCond; auto.
+  - apply CondEta; auto.
+  - apply CondCond; auto.
+  - apply CtxEta; auto.
+  - apply CtxThen; auto.
+  - apply CtxElse; auto.
 Qed.
 
 Lemma fatsemi_End : forall C, (C;;End) = C.
+Proof.
 induction C; simpl; auto.
 + rewrite IHC; auto.
 + rewrite IHC1; rewrite IHC2; auto.
